now free of cheats

src/tools/wp/bir_wp_simpLib.sml
@@ -101,6 +101,9 @@ struct
 
 
 
+
+
+
   val get_concl_lhs = fst o dest_eq o concl;
   val get_concl_rhs = snd o dest_eq o concl;
 
@@ -111,6 +114,61 @@ struct
 
 
   val helper_thm = prove (``!x s t. t UNION (x INSERT s) = if x IN t then t UNION s else (x INSERT t) UNION s``, METIS_TAC [pred_setTheory.INSERT_UNION, pred_setTheory.UNION_COMM, pred_setTheory.INSERT_UNION_EQ]);
+
+
+
+
+
+
+
+
+
+
+
+
+      fun well_typed_conv varexps_thms =
+        let
+(* conversion for welltyped-check *)
+          val simp_conv_for_bir_var_set_is_well_typed0 = SIMP_CONV (std_ss++pred_setSimps.PRED_SET_ss++HolBACoreSimps.holBACore_ss) ([bir_vars_of_exp_def, bir_exp_subst1_USED_VARS, bir_exp_and_def, bir_exp_imp_def, bir_exp_or_def, bir_exp_not_def, bir_exp_varsubst_USED_VARS, bir_exp_varsubst_introduced_vars_REWRS, finite_mapTheory.FDOM_FEMPTY, finite_mapTheory.FDOM_FUPDATE, bir_exp_varsubst1_def]@varexps_thms);
+          val simp_conv_for_bir_var_set_is_well_typed1 = SIMP_CONV (std_ss++stringSimps.STRING_ss++string_ss++char_ss) []; (* TODO: this has to be touched again, new expressions may contain varsubst *)
+          val simp_conv_for_bir_var_set_is_well_typed2 = computeLib.RESTR_EVAL_CONV [``bir_var_set_is_well_typed``];
+          val simp_conv_for_bir_var_set_is_well_typed3 = SIMP_CONV pure_ss [GSYM listTheory.LIST_TO_SET, bir_var_set_is_well_typed_REWRS];
+(*      val simp_conv_for_bir_var_set_is_well_typed4 = SIMP_CONV list_ss [bir_var_name_def, bir_var_type_def];*)
+
+          val simp_conv_for_bir_var_set_is_well_typed =
+                     simp_conv_for_bir_var_set_is_well_typed0 THENC
+                     simp_conv_for_bir_var_set_is_well_typed1 THENC
+                     (
+                    (RAND_CONV (REWRITE_CONV [pred_setTheory.INSERT_UNION_EQ, pred_setTheory.UNION_EMPTY])) THENC
+
+                    REPEATC (
+                      (fn x => REWRITE_CONV [Once helper_thm] x) THENC
+                      ((RATOR_CONV o LAND_CONV) ((REWRITE_CONV [pred_setTheory.IN_INSERT]) THENC
+                                                 (SIMP_CONV (std_ss++HolBACoreSimps.holBACore_ss++stringSimps.STRING_ss++string_ss++char_ss) [pred_setTheory.NOT_IN_EMPTY])))
+                    ) THENC
+
+                    REWRITE_CONV [pred_setTheory.UNION_EMPTY]
+                     ) THENC
+                     (REWRITE_CONV [GSYM listTheory.LIST_TO_SET]) THENC
+                     (REPEATC (
+                        (fn x => REWRITE_CONV [Once bir_var_set_is_well_typed_REWRS] x) THENC
+                        (LAND_CONV EVAL) THENC
+                        (REWRITE_CONV [])
+                     )) THENC
+                     (REWRITE_CONV [bir_var_set_is_well_typed_REWRS]);
+        in
+          simp_conv_for_bir_var_set_is_well_typed
+        end;
+
+
+
+
+
+
+
+
+
+
 
   fun preproc_vars_thm useEval acc def_thm =
     let
@@ -179,7 +237,7 @@ for debugging:
   val varexps_thms = varexps_thms@(!varexps_prems_only);
 *)
 
-  val enableCheats = true;
+  val enableCheats = false;
   val printRuleName = false;
   fun enterRule rulename =
               if (printRuleName) then (
@@ -253,63 +311,6 @@ for debugging:
       val e1_new = (snd o simp_extract o get_concl_rhs) thm_2a;
       val e2_new = (snd o simp_extract o get_concl_rhs) thm_2b;
 
-(*
-      fun prove_well_typed () =
-        let
-(* conversion for welltyped-check *)
-          val simp_conv_for_bir_var_set_is_well_typed0 = SIMP_CONV (std_ss++pred_setSimps.PRED_SET_ss++HolBACoreSimps.holBACore_ss) ([bir_vars_of_exp_def, bir_exp_subst1_USED_VARS, bir_exp_and_def, bir_exp_imp_def, bir_exp_or_def, bir_exp_not_def, bir_exp_varsubst_USED_VARS, bir_exp_varsubst_introduced_vars_REWRS, finite_mapTheory.FDOM_FEMPTY, finite_mapTheory.FDOM_FUPDATE, bir_exp_varsubst1_def]@varexps_thms);
-          val simp_conv_for_bir_var_set_is_well_typed1 = SIMP_CONV (std_ss++stringSimps.STRING_ss++string_ss++char_ss) []; (* TODO: this has to be touched again, new expressions may contain varsubst *)
-          val simp_conv_for_bir_var_set_is_well_typed2 = computeLib.RESTR_EVAL_CONV [``bir_var_set_is_well_typed``];
-          val simp_conv_for_bir_var_set_is_well_typed3 = SIMP_CONV pure_ss [GSYM listTheory.LIST_TO_SET, bir_var_set_is_well_typed_REWRS];
-(*      val simp_conv_for_bir_var_set_is_well_typed4 = SIMP_CONV list_ss [bir_var_name_def, bir_var_type_def];*)
-
-          val simp_conv_for_bir_var_set_is_well_typed =
-                     simp_conv_for_bir_var_set_is_well_typed0 THENC
-                     simp_conv_for_bir_var_set_is_well_typed1 THENC
-                     (
-                    (RAND_CONV (REWRITE_CONV [pred_setTheory.INSERT_UNION_EQ, pred_setTheory.UNION_EMPTY])) THENC
-
-                    REPEATC (
-                      (fn x => REWRITE_CONV [Once helper_thm] x) THENC
-                      ((RATOR_CONV o LAND_CONV) ((REWRITE_CONV [pred_setTheory.IN_INSERT]) THENC
-                                                 (SIMP_CONV (std_ss++HolBACoreSimps.holBACore_ss++stringSimps.STRING_ss++string_ss++char_ss) [pred_setTheory.NOT_IN_EMPTY])))
-                    ) THENC
-
-                    REWRITE_CONV [pred_setTheory.UNION_EMPTY]
-                     ) THENC
-                     (REWRITE_CONV [GSYM listTheory.LIST_TO_SET]) THENC
-                     (REPEATC (
-                        (fn x => REWRITE_CONV [Once bir_var_set_is_well_typed_REWRS] x) THENC
-                        (LAND_CONV EVAL) THENC
-                        (REWRITE_CONV [])
-                     )) THENC
-                     (REWRITE_CONV [bir_var_set_is_well_typed_REWRS]);
-(*          val thm_2c1 = simp_conv_for_bir_var_set_is_well_typed term_2c2;*)
-
-(*
-          val simp_conv_for_bir_var_set_is_well_typed =
-                     simp_conv_for_bir_var_set_is_well_typed0 THENC
-                     simp_conv_for_bir_var_set_is_well_typed1 THENC
-                     simp_conv_for_bir_var_set_is_well_typed2 THENC
-                     simp_conv_for_bir_var_set_is_well_typed3 THENC
-                     EVAL;
-*)
-
-          (*val timer_start = Lib.start_time ();*)
-          val thm_2c1 = simp_conv_for_bir_var_set_is_well_typed term_2c;
-          val term_2c2 = ``bir_var_set_is_well_typed ((bir_vars_of_exp ^prem) UNION (bir_vars_of_exp ^e1_new) UNION (bir_vars_of_exp ^e2_new))``;
-          val thm_2c2 = simp_conv_for_bir_var_set_is_well_typed term_2c2;
-          val thm_2c = TRANS thm_2c1 (GSYM thm_2c2);
-          (*val _ = Lib.end_time timer_start;*)
-        in
-          thm_2c
-        end;
-
-      fun prove_well_typed_cheat () = prove(mk_eq (term_2c, ``bir_var_set_is_well_typed ((bir_vars_of_exp ^prem) UNION (bir_vars_of_exp ^e1_new) UNION (bir_vars_of_exp ^e2_new))``), cheat);
-
-      val prove_well_typed = if enableCheats then prove_well_typed_cheat else prove_well_typed;
-      val thm_2c = prove_well_typed ();
-*)
       val thm_2c = if is_some extra_wt_varset
         then
           (MATCH_MP (MATCH_MP bir_wp_simp_varset_and_helper2_thm wt_preleft) wt_postright)
@@ -320,12 +321,6 @@ for debugging:
           intrRule rulename;
           raise UNCHANGED_bir_wp_simp_step_CONV
         );
-(*
-val dbg_def_1 = Define `debug_def_wpsimp_1 = ^prem`;
-val dbg_def_2 = Define `debug_def_wpsimp_2 = ^e1_new`;
-val dbg_def_3 = Define `debug_def_wpsimp_3 = ^e2_new`;
-val thm_2_dbg = REWRITE_CONV [GSYM dbg_def_1, GSYM dbg_def_2, GSYM dbg_def_3] (get_concl_rhs thm_2);
-*)
 
       val thm_3 = REWRITE_CONV [GSYM bir_wp_simp_taut_and_thm] (get_concl_rhs thm_2);
       val thm_out = TRANS (TRANS thm_1 thm_2) thm_3;
@@ -454,7 +449,7 @@ val thm_2_dbg = REWRITE_CONV [GSYM dbg_def_1, GSYM dbg_def_2, GSYM dbg_def_3] (g
       val wt_thm_in = REWRITE_CONV [def_thm] (simp_construct_wt (prem, term) extra_wt_varset);
       val _ = exitRule rulename;
     in
-      recStepFun (thm_in, wt_thm_in) extra_wt_varset
+      recStepFun (thm_in, wt_thm_in) extra_wt_varset (EQ_MP wt_thm_in wt0_thm)
     end;
 
 
@@ -483,7 +478,7 @@ val thm_2_dbg = REWRITE_CONV [GSYM dbg_def_1, GSYM dbg_def_2, GSYM dbg_def_3] (g
       val wt_thm_in = REWRITE_CONV [thm_1a] (simp_construct_wt (prem, term) extra_wt_varset);
       val _ = exitRule rulename;
     in
-      recStepFun (thm_in, wt_thm_in) extra_wt_varset
+      recStepFun (thm_in, wt_thm_in) extra_wt_varset (EQ_MP wt_thm_in wt0_thm)
     end;
 
 
@@ -519,7 +514,7 @@ val thm_2_dbg = REWRITE_CONV [GSYM dbg_def_1, GSYM dbg_def_2, GSYM dbg_def_3] (g
       val wt_thm_in = REWRITE_CONV [thm_2] (simp_construct_wt (prem, term) extra_wt_varset);
       val _ = exitRule rulename;
     in
-      recStepFun (thm_in, wt_thm_in) extra_wt_varset
+      recStepFun (thm_in, wt_thm_in) extra_wt_varset (EQ_MP wt_thm_in wt0_thm)
     end;
 
 
@@ -555,7 +550,7 @@ val thm_2_dbg = REWRITE_CONV [GSYM dbg_def_1, GSYM dbg_def_2, GSYM dbg_def_3] (g
           val wt_thm_in = REWRITE_CONV [thm_2] (simp_construct_wt (prem, term) extra_wt_varset);
           val _ = exitRule rulename;
         in
-          recStepFun (thm_in, wt_thm_in) extra_wt_varset
+          recStepFun (thm_in, wt_thm_in) extra_wt_varset (EQ_MP wt_thm_in wt0_thm)
         end
       else
         let
@@ -784,7 +779,7 @@ EMPTY UNION {BVar "MEM" (BType_Mem Bit64 Bit8); BVar "R0_wp_10" (BType_Imm Bit64
 
           val _ = exitRule rulename;
         in
-          recStepFun (thm_in, wt_thm_in) extra_wt_varset
+          recStepFun (thm_in, wt_thm_in) extra_wt_varset (EQ_MP wt_thm_in wt0_thm)
         end
     end;
 
@@ -834,7 +829,7 @@ EMPTY UNION {BVar "MEM" (BType_Mem Bit64 Bit8); BVar "R0_wp_10" (BType_Imm Bit64
       val wt_thm_in = REWRITE_CONV [thm_1] (simp_construct_wt (prem, term) extra_wt_varset);
       val _ = exitRule rulename;
     in
-      recStepFun (thm_in, wt_thm_in) extra_wt_varset
+      recStepFun (thm_in, wt_thm_in) extra_wt_varset (EQ_MP wt_thm_in wt0_thm)
     end;
 
 
@@ -875,9 +870,9 @@ EMPTY UNION {BVar "MEM" (BType_Mem Bit64 Bit8); BVar "R0_wp_10" (BType_Imm Bit64
   fun bir_wp_simp_step_CONV useBigstep (varexps_thms:thm list) goalterm extra_wt_varset wt0_thm =
     let
       val rec_step_CONV = bir_wp_simp_step_CONV useBigstep;
-      fun recStepFun (thm_in, wt_thm_in) extra_wt_varset = if useBigstep then
+      fun recStepFun (thm_in, wt_thm_in) extra_wt_varset wt0_thm = if useBigstep then
                          let
-                           val (thm_out, wt_thm_out) = rec_step_CONV varexps_thms (get_concl_rhs thm_in) extra_wt_varset (EQ_MP wt_thm_in wt0_thm);
+                           val (thm_out, wt_thm_out) = rec_step_CONV varexps_thms (get_concl_rhs thm_in) extra_wt_varset wt0_thm;
                          in
                            (TRANS thm_in thm_out, TRANS wt_thm_in wt_thm_out)
                          end
@@ -1005,8 +1000,8 @@ val lbl_list = (gen_lbl_list o snd o dest_eq o concl) aes_wps1_def;
 val varexps_thms = preproc_vars [] (tl (rev lbl_list));
 
 
-val take_all = true;
-val i = 17; (* 2, 3, 17, 20, 200, all *)
+val take_all = false;
+val i = 30; (* 2, 3, 17, 20, 200, all *)
 
 val i_min = 1;
 val i_max = (List.length lbl_list) - 1;
@@ -1025,15 +1020,22 @@ val def_const = (fst o dest_eq o concl) def_thm;
 val btautology = ``BExp_Const (Imm1 1w)``;
 val prem_init = ``^btautology``; (* have another premise here *)
 
-val wt0_thm = ASSUME (simp_construct_wt (simp_extract goalterm) NONE);
+
 val goalterm = ``bir_exp_is_taut (bir_exp_imp ^prem_init (bir_exp_varsubst FEMPTY ^def_const))``;
 
+
+(*ASSUME (simp_construct_wt (simp_extract goalterm) NONE);*)
+val wt0_thm = prove (``^(simp_construct_wt (simp_extract goalterm) NONE)``,
+  CONV_TAC (well_typed_conv varexps_thms)
+);
 
 val timer_start = Lib.start_time ();
 val (simp_thm,wt_eq_thm) = bir_wp_simp_CONV varexps_thms goalterm wt0_thm;
 val _ = Lib.end_time timer_start;
 
-
+(*
+hyp simp_thm;
+*)
 
 (*
 ------------ stepwise debugging
