src/tools/wp/examples/aes/aesSimpWpScript.sml
@@ -10,7 +10,6 @@ open bir_wp_simpLib;
 val _ = new_theory "aesSimpWp";
 
 
-(*
 
 val lbl_list = (gen_lbl_list o snd o dest_eq o concl) aes_wps1_def;
 
@@ -19,8 +18,8 @@ val varexps_thms = preproc_vars [] (tl (rev lbl_list));
 
 
 (* provide the number of arm instructions to take for the simplification, counted from the end of the computed block *)
-val take_all = true;
-val i = 2; (*60 - 230;*)
+val take_all = false;
+val i = 30; (*60 - 230;*)
 
 val i_min = 1;
 val i_max = (List.length lbl_list) - 1;
@@ -41,14 +40,25 @@ val prem_init = ``^btautology``; (* have another premise here *)
 
 val goalterm = ``bir_exp_is_taut (bir_exp_imp ^prem_init (bir_exp_varsubst FEMPTY ^def_const))``;
 
+(*ASSUME (simp_construct_wt (simp_extract goalterm) NONE);*)
+val wt0_thm = prove (``^(simp_construct_wt (simp_extract goalterm) NONE)``,
+  CONV_TAC (well_typed_conv varexps_thms)
+);
+
+
 val timer_start = Lib.start_time ();
-val simp_thm = bir_wp_simp_CONV varexps_thms goalterm;
+val (simp_thm,wt_thm) = bir_wp_simp_CONV varexps_thms goalterm wt0_thm;
 val _ = Lib.end_time timer_start;
 
 
-val _ = save_thm("aes_wp_taut_thm", simp_thm);
+val wp_simp_term = (snd o dest_comb o snd o dest_comb o snd o dest_eq o concl) simp_thm;
+val wp_simp_def = Define `wp_simp_def = ^wp_simp_term`;
 
-*)
+
+val aes_wp_taut_thm = save_thm("aes_wp_taut_thm", REWRITE_RULE [GSYM wp_simp_def] simp_thm);
+val aes_wp_wt_thm = save_thm("aes_wp_wt_thm", REWRITE_RULE [GSYM wp_simp_def] wt_thm);
+
+
 
 
 val _ = export_theory();
